Remove old files

src/Matrix.fst
@@ -4,117 +4,148 @@ open Scalar
 open Vector
 open MatrixType
 
-(* destructors *)
-assume val destruct : #n:pos{n >= 2} -> m:mat n ->
-  c:cvec (n-1) & a:num & b:rvec (n-1) & d:mat (n-1){
-    (lower m ==> lower d /\ zero_vec b) /\
-    (upper m ==> upper d /\ zero_vec c) /\
-    (unit_diag m ==> one a /\ unit_diag d) /\
-    (pos_diag m ==> posr a /\ pos_diag d) /\
-    (nnz_diag m ==> nnz a /\ nnz_diag d) /\
-    (top_left_nnz m ==> nnz a) /\
-    (rowsdd m ==> rowsdd d) /\
-    (spd m ==> spd d /\ posr a)
-  }
-
-(* augmenters *)
-assume val augment : #n:pos{n >= 2} -> m:mat (n-1) ->
-  c:cvec (n-1) -> a:num -> b:rvec (n-1) -> d:mat n{
-    (lower m /\ zero_vec b ==> lower d) /\
-    (upper m /\ zero_vec c ==> upper d) /\
-    (unit_diag m /\ one a ==> unit_diag d) /\
-    (pos_diag m /\ posr a ==> pos_diag d) /\
-    (nnz_diag m /\ nnz a ==> nnz_diag d) /\
-    (perm m /\ zero_vec c /\ one a /\ zero_vec b ==> perm d)
-  }
-
-(* augment id with zero vec *)
-assume val augment_identity_zero : #m:pos -> #n:pos{n >= 2} ->
-  Lemma (requires n = m + 1)
-        (ensures augment #n _id_mat _zero_cvec _one _zero_rvec == _id_mat)
-        [SMTPat (augment #n (_id_mat #m) (_zero_cvec #m) _one (_zero_rvec #m))]
-
-(* destructing then augmenting recovers the original matrix *)
-assume val augment_destruct_inv : #n:pos{n >= 2} -> m:mat n ->
-  Lemma (ensures (let (|c, a, b, d|) = destruct m in augment d c a b == m))
-        [SMTPat (destruct m)]
-
 (* matrix-vector mul *)
-assume val mat_vec_mul : #n:pos -> m:mat n -> c1:cvec n -> c2:cvec n{
-  (identity m ==> c1 == c2) /\ (zero_vec c1 ==> zero_vec c2)
-}
+let rec mat_vec_mul (#n: pos) (m: mat n) (v: cvec n) : cvec n =
+  match m with
+  | Mat1 a ->
+    let Vec1 x = v in Vec1 (scalar_mul a x)
+  | MatN m' c a b ->
+    let VecN v' vn = v in
+    VecN (vec_add (mat_vec_mul m' v') (vec_scalar_mul c vn))
+         (scalar_add (inner_prod b v') (scalar_mul a vn))
 
-assume val vec_mat_mul : #n:pos -> r1:rvec n -> m:mat n -> r2:rvec n{
-  (identity m ==> r1 == r2) /\ (zero_vec r1 ==> zero_vec r2)
-}
+(* row-vector times matrix *)
+let rec vec_mat_mul (#n: pos) (r: rvec n) (m: mat n) : rvec n =
+  match m with
+  | Mat1 a ->
+    let Vec1 x = r in Vec1 (scalar_mul x a)
+  | MatN m' c a b ->
+    let VecN r' rn = r in
+    VecN (vec_add (vec_mat_mul r' m') (vec_scalar_mul b rn))
+         (scalar_add (inner_prod r' c) (scalar_mul rn a))
 
-(* mul by neg vec *)
-assume val mat_vec_mul_neg : #n:pos -> m:mat n -> c:cvec n ->
-  Lemma (mat_vec_mul m (neg c) == neg (mat_vec_mul m c))
-        [SMTPat (mat_vec_mul m (neg c))]
+assume val mat_vec_mul_id (#n: pos) (m: mat n) (v: cvec n)
+    : Lemma (requires is_id m) (ensures mat_vec_mul m v == v)
+      [SMTPat (mat_vec_mul m v)]
 
-(* m * (a * c) == a * (m * c) *)
-assume val mat_vec_mul_scalar : #n:pos -> m:mat n -> c:cvec n -> a:num ->
-  Lemma (mat_vec_mul m (vec_scalar_mul c a) == vec_scalar_mul (mat_vec_mul m c) a)
-  [SMTPat (mat_vec_mul m (vec_scalar_mul c a))]
+let rec mat_vec_mul_zero_vec (#n: pos) (m: mat n) (v: cvec n)
+    : Lemma (requires is_zero_vec v) (ensures is_zero_vec (mat_vec_mul m v))
+      [SMTPat (mat_vec_mul m v)] =
+  match m with
+  | Mat1 _ -> let Vec1 _ = v in ()
+  | MatN m' _ _ _ ->
+    let VecN v' _ = v in
+    mat_vec_mul_zero_vec m' v'
+
+assume val vec_mat_mul_id (#n: pos) (r: rvec n) (m: mat n)
+    : Lemma (requires is_id m) (ensures vec_mat_mul r m == r)
+      [SMTPat (vec_mat_mul r m)]
+
+let rec vec_mat_mul_zero_vec (#n: pos) (r: rvec n) (m: mat n)
+    : Lemma (requires is_zero_vec r) (ensures is_zero_vec (vec_mat_mul r m))
+      [SMTPat (vec_mat_mul r m)] =
+  match m with
+  | Mat1 _ -> let Vec1 _ = r in ()
+  | MatN m' _ _ _ ->
+    let VecN r' _ = r in
+    vec_mat_mul_zero_vec r' m'
+
+assume val mat_vec_mul_vec_neg (#n: pos) (m: mat n) (c: cvec n)
+    : Lemma (mat_vec_mul m (vec_neg c) == vec_neg (mat_vec_mul m c))
+      [SMTPat (mat_vec_mul m (vec_neg c))]
+
+assume val mat_vec_mul_scalar (#n: pos) (m: mat n) (c: cvec n) (a: num)
+    : Lemma (mat_vec_mul m (vec_scalar_mul c a) == vec_scalar_mul (mat_vec_mul m c) a)
+      [SMTPat (mat_vec_mul m (vec_scalar_mul c a))]
 
 (* outer product *)
-assume val outer_prod : #n:pos -> c:cvec n -> r:rvec n -> m:mat n{
-  (zero_vec c \/ zero_vec r) ==> zero_mat m
-}
+assume val outer_prod (#n: pos) (c: cvec n) (r: rvec n)
+    : m: mat n {(is_zero_vec c \/ is_zero_vec r) ==> is_zero_mat m}
 
-(* outer prod of scalar div *)
-assume val outer_prod_div_comm : #n:pos -> c:cvec n -> b:rvec n -> l:num{nnz l} ->
-  Lemma (outer_prod c (vec_scalar_div b l) == outer_prod (vec_scalar_div c l) b)
-  [SMTPat (outer_prod c (vec_scalar_div b l))]
+assume val outer_prod_div_comm (#n: pos) (c: cvec n) (b: rvec n) (l: num{is_nnz l})
+    : Lemma (outer_prod c (vec_scalar_div b l) == outer_prod (vec_scalar_div c l) b)
+      [SMTPat (outer_prod c (vec_scalar_div b l))]
 
-(* adding matrices *)
-assume val mat_add : #n:pos -> m1:mat n -> m2:mat n -> m3:mat n{
-  (zero_mat m1 ==> m2 == m3) /\ (zero_mat m2 ==> m1 == m3)
-}
+(* matrix addition *)
+let rec mat_add (#n: pos) (m1 m2: mat n) : mat n =
+  match m1 with
+  | Mat1 a -> let Mat1 b = m2 in Mat1 (scalar_add a b)
+  | MatN m1' col1 corner1 row1 ->
+    let MatN m2' col2 corner2 row2 = m2 in
+    MatN (mat_add m1' m2') (vec_add col1 col2) (scalar_add corner1 corner2) (vec_add row1 row2)
 
-assume val mat_sub : #n:pos -> m1:mat n -> m2:mat n -> m3:mat n{
-  mat_add m2 m3 == m1
-}
+let rec mat_add_zero_l (#n: pos) (m1 m2: mat n)
+    : Lemma (requires is_zero_mat m1) (ensures mat_add m1 m2 == m2) [SMTPat (mat_add m1 m2)] =
+  match m1 with
+  | Mat1 _ -> let Mat1 _ = m2 in ()
+  | MatN m1' _ _ _ ->
+    let MatN m2' _ _ _ = m2 in
+    mat_add_zero_l m1' m2'
+
+let rec mat_add_zero_r (#n: pos) (m1 m2: mat n)
+    : Lemma (requires is_zero_mat m2) (ensures mat_add m1 m2 == m1) [SMTPat (mat_add m1 m2)] =
+  match m1 with
+  | Mat1 _ -> let Mat1 _ = m2 in ()
+  | MatN m1' _ _ _ ->
+    let MatN m2' _ _ _ = m2 in
+    mat_add_zero_r m1' m2'
+
+(* matrix negation *)
+let rec mat_neg (#n: pos) (m: mat n) : mat n =
+  match m with
+  | Mat1 a -> Mat1 (scalar_neg a)
+  | MatN m' c a b -> MatN (mat_neg m') (vec_neg c) (scalar_neg a) (vec_neg b)
+
+(* matrix subtraction *)
+let mat_sub (#n: pos) (m1 m2: mat n) : mat n = mat_add m1 (mat_neg m2)
+
+assume val mat_add_sub_cancel (#n: pos) (m1 m2: mat n)
+    : Lemma (mat_add m2 (mat_sub m1 m2) == m1)
+      [SMTPat (mat_add m2 (mat_sub m1 m2))]
 
 (* schur complement *)
-let schur1 (#n:pos) (d:mat n) (c:cvec n) (a:num{nnz a}) (b:rvec n) : mat n =
+// let schur1 (#n: pos{n >= 2}) (m: mat n{rowsdd m}) : mat n = 
+//   match m with 
+//   | MatN #n m' c a b -> 
+//     assert (m' : mat n); 
+//     mat_sub m' (outer_prod (vec_scalar_div c a) b)
+
+
+let schur1 (#n: pos) (d: mat n) (c: cvec n) (a: num{is_nnz a}) (b: rvec n) : mat n =
   mat_sub d (outer_prod (vec_scalar_div c a) b)
 
-assume val schur1_spd : #n:pos -> d:mat n -> c:cvec n -> a:num{nnz a} -> b:rvec n ->
-  Lemma (requires spd (augment #(n+1) d c a b))
-        (ensures spd (schur1 d c a b))
-        [SMTPat (schur1 d c a b)]
+assume val schur1_spd (#n: pos) (d: mat n) (c: cvec n) (a: num{is_nnz a}) (b: rvec n)
+    : Lemma (requires spd (MatN d c a b)) (ensures spd (schur1 d c a b)) [SMTPat (schur1 d c a b)]
 
-assume val schur1_rowsdd : #n:pos -> d:mat n -> c:cvec n -> a:num{nnz a} -> b:rvec n ->
-  Lemma (requires rowsdd (augment #(n+1) d c a b))
-        (ensures rowsdd (schur1 d c a b))
-        [SMTPat (schur1 d c a b)]
+assume val schur1_rowsdd (#n: pos) (d: mat n) (c: cvec n) (a: num{is_nnz a}) (b: rvec n)
+    : Lemma (requires rowsdd (MatN d c a b))
+      (ensures rowsdd (schur1 d c a b))
+      [SMTPat (schur1 d c a b)]
 
-assume val schur1_inv : #n:pos -> d:mat n -> c:cvec n -> a:num{nnz a} -> b:rvec n ->
-  Lemma (requires inv (augment #(n+1) d c a b))
-        (ensures inv (schur1 d c a b))
-        [SMTPat (schur1 d c a b)]
+assume val schur1_inv (#n: pos) (d: mat n) (c: cvec n) (a: num{is_nnz a}) (b: rvec n)
+    : Lemma (requires inv (MatN d c a b)) (ensures inv (schur1 d c a b)) [SMTPat (schur1 d c a b)]
 
 (* transpose *)
-assume val transpose : #n:pos -> mat n -> mat n
+let rec transpose (#n: pos) (m: mat n) : mat n =
+  match m with
+  | Mat1 a -> Mat1 a
+  | MatN m' c a b -> MatN (transpose m') (vec_trans b) a (vec_trans c)
 
-assume val transpose_involutive : #n:pos -> m:mat n ->
-  Lemma (transpose (transpose m) == m) [SMTPat (transpose (transpose m))]
-
-assume val transpose_augment : #n:pos{n >= 2} -> m:mat (n-1) -> 
-  c:cvec (n-1) -> a:num -> b:rvec (n-1) ->
-  Lemma (transpose (augment m c a b) == augment (transpose m) (trans_vec b) a (trans_vec c))
-  [SMTPat (transpose (augment m c a b))]
+let rec transpose_involutive (#n: pos) (m: mat n)
+    : Lemma (transpose (transpose m) == m) [SMTPat (transpose (transpose m))] =
+  match m with
+  | Mat1 _ -> ()
+  | MatN m' _ _ _ -> transpose_involutive m'
 
 (* symmetry *)
-let symmetric (#n:pos) (m:mat n) : prop = m == transpose m
+let symmetric (#n: pos) (m: mat n) : prop = m == transpose m
 
-assume val destruct_symmetric : #n:pos{n >= 2} -> m:mat n ->
-  Lemma (requires symmetric m)
-        (ensures (let (|c, a, b, d|) = destruct m in
-                  trans_vec c == b /\ trans_vec b == c))
-        [SMTPat (destruct m)]
+assume val one_by_one_sym : m:mat 1 -> Lemma (symmetric m) [SMTPat (symmetric m)]
 
-assume val spd_symmetric : #n:pos -> m:mat n ->
-  Lemma (requires spd m) (ensures symmetric m) [SMTPat (spd m)]
+// let matN_symmetric (#n: pos) (m: mat n) (col: cvec n) (corner: num) (row: rvec n)
+//     : Lemma (requires symmetric (MatN m col corner row))
+//       (ensures vec_trans col == row /\ vec_trans row == col)
+//       [SMTPat (symmetric (MatN m col corner row))] = ()
+
+assume val spd_symmetric (#n: pos) (m: mat n)
+    : Lemma (requires spd m) (ensures symmetric m) [SMTPat (spd m)]
