src/MatrixType.fst
@@ -1,61 +1,114 @@
 module MatrixType
 
 open Scalar
+open Vector
 
 (* square matrices *)
-assume type mat : pos -> Type
+noeq type mat : pos -> Type =
+  | Mat1 : num -> mat 1
+  | MatN : #n: pos -> mat n -> cvec n -> num -> rvec n -> mat (n + 1)
 
 (* shapes *)
-assume val lower : #n:pos -> mat n -> prop
-assume val upper : #n:pos -> mat n -> prop
-let diagonal (#n:pos) (m:mat n) : prop = lower m /\ upper m
+let rec lower (#n: pos) (m: mat n) : prop =
+  match m with
+  | Mat1 _ -> True
+  | MatN m' _ _ row -> lower m' /\ is_zero_vec row
+
+let rec upper (#n: pos) (m: mat n) : prop =
+  match m with
+  | Mat1 _ -> True
+  | MatN m' col _ _ -> upper m' /\ is_zero_vec col
+
+assume val one_by_one_lower : m:mat 1 -> Lemma (lower m) [SMTPat (lower m)]
+assume val one_by_one_upper : m:mat 1 -> Lemma (upper m) [SMTPat (upper m)]
+
+let diagonal (#n: pos) (m: mat n) : prop = lower m /\ upper m
 
 (* what's on the diagonal *)
-assume val unit_diag : #n:pos -> mat n -> prop
-assume val nnz_diag  : #n:pos -> mat n -> prop
-assume val pos_diag  : #n:pos -> mat n -> prop
+let rec unit_diag (#n: pos) (m: mat n) : prop =
+  match m with
+  | Mat1 a -> is_one a
+  | MatN m' _ corner _ -> unit_diag m' /\ is_one corner
 
-assume val pos_diag_nnz : #n:pos -> m:mat n ->
-  Lemma (requires pos_diag m) (ensures nnz_diag m) [SMTPat (pos_diag m)]
+let rec nnz_diag (#n: pos) (m: mat n) : prop =
+  match m with
+  | Mat1 a -> is_nnz a
+  | MatN m' _ corner _ -> nnz_diag m' /\ is_nnz corner
 
-assume val unit_diag_pos : #n:pos -> m:mat n ->
-  Lemma (requires unit_diag m) (ensures pos_diag m) [SMTPat (unit_diag m)]
+let rec pos_diag (#n: pos) (m: mat n) : prop =
+  match m with
+  | Mat1 a -> is_pos a
+  | MatN m' _ corner _ -> pos_diag m' /\ is_pos corner
+
+let rec pos_diag_nnz (#n: pos) (m: mat n)
+    : Lemma (requires pos_diag m) (ensures nnz_diag m) [SMTPat (pos_diag m)] =
+  match m with
+  | Mat1 _ -> ()
+  | MatN m' _ _ _ -> pos_diag_nnz m'
+
+let rec unit_diag_pos (#n: pos) (m: mat n)
+    : Lemma (requires unit_diag m) (ensures pos_diag m) [SMTPat (unit_diag m)] =
+  match m with
+  | Mat1 _ -> ()
+  | MatN m' _ _ _ -> unit_diag_pos m'
 
 (* properties *)
-assume val rowsdd : #n:pos -> mat n -> prop
-assume val spd    : #n:pos -> mat n -> prop
-assume val inv    : #n:pos -> mat n -> prop
+assume val rowsdd: #n: pos -> mat n -> prop
+assume val spd: #n: pos -> mat n -> prop
+assume val inv: #n: pos -> mat n -> prop
 
-assume val spd_pos_diag : #n:pos -> m:mat n ->
-  Lemma (requires spd m) (ensures pos_diag m) [SMTPat (spd m)]
+assume val spd_pos_diag (#n: pos) (m: mat n) : Lemma (requires spd m) (ensures pos_diag m) [SMTPat (spd m)]
 
-assume val rowsdd_nnz_diag : #n:pos -> m:mat n ->
-  Lemma (requires rowsdd m) (ensures nnz_diag m) [SMTPat (rowsdd m)]
+assume val rowsdd_nnz_diag (#n: pos) (m: mat n)
+    : Lemma (requires rowsdd m) (ensures nnz_diag m) [SMTPat (rowsdd m)]
+
+assume val destruct_rowsdd (#n: pos{n >= 2}) (m: mat n) :
+    Lemma (requires rowsdd m) (ensures (let MatN m' b a c = m in rowsdd m' /\ is_nnz a)) [SMTPat (rowsdd m)]
+
+assume val destruct_spd (#n: pos{n >= 2}) (m: mat n) :
+    Lemma (requires spd m) (ensures (let MatN m' b a c = m in spd m' /\ is_pos a)) [SMTPat (spd m)]
+
+assume val inv_1x1_nnz_diag (m:mat 1) :
+  Lemma (requires inv m) (ensures nnz_diag m) [SMTPat (inv (m <: mat 1))]
 
 (* shorthands *)
-let unit_lower (#n:pos) (m:mat n) : prop = lower m /\ unit_diag m
+let unit_lower (#n: pos) (m: mat n) : prop = lower m /\ unit_diag m
 
 (* identity *)
-assume val _id_mat : #n:pos -> m:mat n{diagonal m /\ unit_diag m}
+let rec id_mat (#n: pos) : mat n =
+  if n = 1 then Mat1 one else MatN (id_mat #(n - 1)) zero_cvec one zero_rvec
 
-let identity (#n:pos) (m:mat n) : prop = m == _id_mat
+let is_id (#n: pos) (m: mat n) : prop = m == id_mat
 
 (* zero matrix *)
-assume val _zero_mat : #n:pos -> mat n
+let rec zero_mat (#n: pos) : mat n =
+  if n = 1
+  then Mat1 zero
+  else MatN (zero_mat #(n - 1)) zero_cvec zero zero_rvec
 
-let zero_mat (#n:pos) (m:mat n) : prop = m == _zero_mat
+let is_zero_mat (#n: pos) (m: mat n) : prop = m == zero_mat
+
+// let rec id_mat_diagonal (#n: pos) : Lemma (diagonal (id_mat #n)) [SMTPat (id_mat #n)] =
+//   if n = 1 then () else id_mat_diagonal #(n - 1)
+
+// let rec id_mat_unit_diag (#n: pos) : Lemma (unit_diag (id_mat #n)) [SMTPat (id_mat #n)] =
+//   if n = 1 then () else id_mat_unit_diag #(n - 1)
 
 (* permutation matrix *)
-assume val perm : #n:pos -> mat n -> prop
+assume val perm: #n: pos -> mat n -> prop
 
-assume val perm_is_inv : #n:pos -> m:mat n ->
-  Lemma (requires perm m) (ensures inv m) [SMTPat (perm m)]
+assume val perm_is_inv (#n: pos) (m: mat n) : Lemma (requires perm m) (ensures inv m) [SMTPat (perm m)]
 
-assume val id_mat_is_perm : #n:pos ->
-  Lemma (perm (_id_mat #n)) [SMTPat (_id_mat #n)]
+assume val id_mat_is_perm (#n: pos) : Lemma (perm (id_mat #n)) [SMTPat (id_mat #n)]
+
+assume val augment_perm (#n: pos) (m: mat n{perm m}) :
+  Lemma (perm (MatN m zero_vec one zero_vec)) [SMTPat (perm m)]
 
 (* top-left entry is nonzero *)
-assume val top_left_nnz : #n:pos -> mat n -> prop
+let top_left_nnz (#n: pos) (m: mat n) : prop =
+  match m with
+  | Mat1 a -> is_nnz a
+  | MatN _ _ corner _ -> is_nnz corner
 
-assume val nnz_diag_top_left : #n:pos -> m:mat n ->
-  Lemma (requires nnz_diag m) (ensures top_left_nnz m) [SMTPat (nnz_diag m)]
+let nnz_diag_top_left (#n: pos) (m: mat n)
+    : Lemma (requires nnz_diag m) (ensures top_left_nnz m) [SMTPat (nnz_diag m)] = ()
