src/Scalar.fst
@@ -2,35 +2,48 @@ module Scalar
 
 assume type num : Type
 
-assume val _one  : num
-assume val _zero : num
+assume val one : num
+assume val zero : num
 
-assume val posr : num -> prop
+assume val is_pos : num -> prop
+let is_one (a: num) : prop = a == one
+let is_zero (a: num) : prop = a == zero
+let is_nnz (a: num) : prop = ~(is_zero a)
+let is_nneg (a: num) : prop = is_pos a \/ is_zero a
 
-let one  (a:num) : prop = a == _one
-let zero (a:num) : prop = a == _zero
-let nnz  (a:num) : prop = ~(zero a)
+assume val one_is_pos (a: num) : Lemma (requires is_one a) (ensures is_pos a) [SMTPat (is_one a)]
 
-assume val one_is_pos : a:num ->
-  Lemma (requires one a) (ensures posr a) [SMTPat (one a)]
+assume val pos_is_nnz (a: num) : Lemma (requires is_pos a) (ensures is_nnz a) [SMTPat (is_pos a)]
 
-assume val pos_is_nnz : a:num ->
-  Lemma (requires posr a) (ensures nnz a) [SMTPat (posr a)]
+(* multiplication *)
+assume val scalar_mul (a1 a2: num) : a3: num
+      { (is_one a1 ==> a3 == a2) /\ (is_one a2 ==> a3 == a1) /\
+        (is_pos a1 /\ is_pos a2 ==> is_pos a3) /\ (is_nnz a1 /\ is_nnz a2 ==> is_nnz a3) /\
+        (is_zero a1 \/ is_zero a2 ==> is_zero a3) }
 
-assume val scalar_mul : a1:num -> a2:num -> a3:num{
-  (one a1 ==> a3 == a2) /\
-  (one a2 ==> a3 == a1) /\
-  (posr a1 /\ posr a2 ==> posr a3) /\
-  (nnz  a1 /\ nnz  a2 ==> nnz  a3) /\
-  (zero a1 \/ zero a2 ==> zero a3)
-}
+(* division *)
+assume val scalar_div (a1: num) (a2: num{is_nnz a2}) : a3: num{scalar_mul a3 a2 == a1}
 
-assume val scalar_add : a1:num -> a2:num -> a3:num{
-  (zero a1 ==> a2 == a3) /\
-  (zero a2 ==> a1 == a3) /\
-  (posr a1 /\ posr a2 ==> posr a3)
-}
+assume val scalar_div_assoc (a: num) (a1: num{is_nnz a1}) (a2: num{is_nnz a2})
+    : Lemma (scalar_div (scalar_div a a1) a2 == scalar_div a (scalar_mul a1 a2))
+      [SMTPat (scalar_div (scalar_div a a1) a2)]
 
-assume val sqrt : a1:num{posr a1} -> a2:num{
-  posr a2 /\ scalar_mul a2 a2 == a1
-}
+(* addition *)
+assume val scalar_add (a1 a2: num) : a3: num
+      { (is_zero a1 ==> a2 == a3) /\ (is_zero a2 ==> a1 == a3) /\
+        (is_pos a1 /\ is_pos a2 ==> is_pos a3) }
+
+(* square root *)
+assume val sqrt (a1: num{is_nneg a1})
+    : a2:num{(is_pos a1 ==> is_pos a2) /\ (is_zero a1 <==> is_zero a2) /\ scalar_mul a2 a2 == a1}
+
+(* negate *)
+assume val scalar_neg (a: num) : b: num
+      { scalar_add a b == zero /\ scalar_add b a == zero /\ (is_zero a ==> is_zero b) /\
+        (is_zero b ==> is_zero a) }
+
+assume val scalar_neg_involutive (a: num)
+    : Lemma (scalar_neg (scalar_neg a) == a) [SMTPat (scalar_neg (scalar_neg a))]
+
+(* subtraction *)
+let scalar_sub (a1 a2: num) : num = scalar_add a1 (scalar_neg a2)
