src/Vector.fst
@@ -2,79 +2,159 @@ module Vector
 
 open Scalar
 
-assume type vec : pos -> Type
+type orient = | Row | Col
+let flip (o: orient) : orient = match o with | Row -> Col | Col -> Row
 
-assume val row : #n:pos -> vec n -> prop
-let col (#n:pos) (v:vec n) : prop = ~(row v)
+noeq type vec : orient -> pos -> Type =
+  | Vec1 : #o: orient -> num -> vec o 1
+  | VecN : #o: orient -> #n: pos -> vec o n -> num -> vec o (n + 1)
 
-let rvec (n:pos) = r:vec n{row r}
-let cvec (n:pos) = c:vec n{col c}
+let row (#n: pos) (v: vec Row n) : prop = True
+let col (#n: pos) (v: vec Col n) : prop = True
 
-let vec_compat (#n:pos) (v1 v2:vec n) : prop =
-  (col v1 /\ col v2) \/ (row v1 /\ row v2)
+let rvec (n: pos) : Type = vec Row n
+let cvec (n: pos) : Type = vec Col n
 
 (* zero vector *)
-assume val _zero_cvec : #n:pos -> cvec n
-assume val _zero_rvec : #n:pos -> rvec n
+let rec zero_vec (#o: orient) (#n: pos) : vec o n =
+  if n = 1 then Vec1 #o zero else VecN (zero_vec #o #(n - 1)) zero
 
-let zero_vec (#n:pos) (v:vec n) : prop =
-  (row v /\ v == _zero_rvec #n) \/ (col v /\ v == _zero_cvec #n)
+let zero_rvec (#n: pos) : rvec n = zero_vec #Row #n
+let zero_cvec (#n: pos) : cvec n = zero_vec #Col #n
+
+let is_zero_vec (#o: orient) (#n: pos) (v: vec o n) : prop = v == zero_vec #o #n
 
 (* add vectors *)
-assume val vec_add : #n:pos -> v1:vec n -> v2:vec n{vec_compat v1 v2} -> v3:vec n{
-  (zero_vec v1 ==> v3 == v2) /\
-  (zero_vec v2 ==> v3 == v1) /\
-  (row v1 <==> row v3)
-}
+let rec vec_add (#o: orient) (#n: pos) (v1 v2: vec o n) : vec o n =
+  match v1 with
+  | Vec1 x -> let Vec1 y = v2 in Vec1 (scalar_add x y)
+  | VecN v1' x -> let VecN v2' y = v2 in VecN (vec_add v1' v2') (scalar_add x y)
+
+let rec vec_add_zero_l (#o: orient) (#n: pos) (v1 v2: vec o n)
+    : Lemma (requires is_zero_vec v1) (ensures vec_add v1 v2 == v2) [SMTPat (vec_add v1 v2)] =
+  match v1 with 
+  | Vec1 _ -> let Vec1 _ = v2 in ()
+  | VecN v1' _ -> let VecN v2' _ = v2 in vec_add_zero_l v1' v2'
+
+let rec vec_add_zero_r (#o: orient) (#n: pos) (v1 v2: vec o n)
+    : Lemma (requires is_zero_vec v2) (ensures vec_add v1 v2 == v1) [SMTPat (vec_add v1 v2)] =
+  match v2 with
+  | Vec1 _ -> let Vec1 _ = v1 in ()
+  | VecN v2' _ -> let VecN v1' _ = v1 in vec_add_zero_r v1' v2'
 
 (* negate a vector *)
-assume val neg : #n:pos -> v1:vec n -> v2:vec n{
-  (row v1 <==> row v2) /\ (zero_vec v1 ==> zero_vec v2)
-}
+let rec vec_neg (#o: orient) (#n: pos) (v: vec o n) : vec o n =
+  match v with
+  | Vec1 x -> Vec1 (scalar_neg x)
+  | VecN v' x -> VecN (vec_neg v') (scalar_neg x)
 
-assume val neg_add_inv_l : #n:pos -> v:vec n ->
-  Lemma (zero_vec (vec_add v (neg v))) [SMTPat (vec_add v (neg v))]
+let rec vec_neg_zero (#o: orient) (#n: pos) (v: vec o n)
+    : Lemma (requires is_zero_vec v) (ensures is_zero_vec (vec_neg v)) [SMTPat (vec_neg v)] =
+  match v with
+  | Vec1 _ -> ()
+  | VecN v' _ -> vec_neg_zero v'
 
-assume val neg_add_inv_r : #n:pos -> v:vec n ->
-  Lemma (zero_vec (vec_add (neg v) v)) [SMTPat (vec_add (neg v) v)]
+let rec vec_neg_add_inv_l (#o: orient) (#n: pos) (v: vec o n)
+    : Lemma (is_zero_vec (vec_add v (vec_neg v))) [SMTPat (vec_add v (vec_neg v))] =
+  match v with
+  | Vec1 _ -> ()
+  | VecN v' _ -> vec_neg_add_inv_l v'
 
-assume val neg_involutive : #n:pos -> v:vec n ->
-  Lemma (neg (neg v) == v) [SMTPat (neg (neg v))]
+let rec vec_neg_add_inv_r (#o: orient) (#n: pos) (v: vec o n)
+    : Lemma (is_zero_vec (vec_add (vec_neg v) v)) [SMTPat (vec_add (vec_neg v) v)] =
+  match v with
+  | Vec1 _ -> ()
+  | VecN v' _ -> vec_neg_add_inv_r v'
 
-(* vector-scalar mult *)
-assume val vec_scalar_mul : #n:pos -> v1:vec n -> a:num -> v2:vec n{
-  (row v1 <==> row v2)
-}
+let rec vec_neg_involutive (#o: orient) (#n: pos) (v: vec o n)
+    : Lemma (vec_neg (vec_neg v) == v) [SMTPat (vec_neg (vec_neg v))] =
+  match v with
+  | Vec1 _ -> ()
+  | VecN v' _ -> vec_neg_involutive v'
 
-assume val vec_scalar_mul_zero : #n:pos -> v:vec n -> a:num ->
-  Lemma (requires zero_vec v) (ensures zero_vec (vec_scalar_mul v a)) 
-  [SMTPat (vec_scalar_mul v a)]
+(* vector-scalar mul *)
+let rec vec_scalar_mul (#o: orient) (#n: pos) (v: vec o n) (a: num) : vec o n =
+  match v with
+  | Vec1 x -> Vec1 (scalar_mul x a)
+  | VecN v' x -> VecN (vec_scalar_mul v' a) (scalar_mul x a)
 
-assume val vec_scalar_mul_one : #n:pos -> v:vec n -> a:num ->
-  Lemma (requires one a) (ensures vec_scalar_mul v a == v) 
-  [SMTPat (vec_scalar_mul v a)]
+let rec vec_scalar_mul_one (#o: orient) (#n: pos) (v: vec o n) (a: num)
+    : Lemma (requires is_one a) (ensures vec_scalar_mul v a == v) [SMTPat (vec_scalar_mul v a)] =
+  match v with
+  | Vec1 _ -> ()
+  | VecN v' _ -> vec_scalar_mul_one v' a
 
-assume val vec_scalar_div : #n:pos -> v1:vec n -> a:num{nnz a} -> v2:vec n{
-  (row v1 <==> row v2) /\ vec_scalar_mul v2 a == v1
-}
+let rec vec_scalar_mul_zero (#o: orient) (#n: pos) (v: vec o n) (a: num)
+    : Lemma (requires is_zero_vec v)
+      (ensures is_zero_vec (vec_scalar_mul v a))
+      [SMTPat (vec_scalar_mul v a)] =
+  match v with
+  | Vec1 _ -> ()
+  | VecN v' _ -> vec_scalar_mul_zero v' a
 
-assume val vec_scalar_div_assoc : #n:pos -> v:vec n -> a1:num{nnz a1} -> a2:num{nnz a2} ->
-  Lemma (vec_scalar_div (vec_scalar_div v a1) a2 == vec_scalar_div v (scalar_mul a1 a2))
-        [SMTPat (vec_scalar_div (vec_scalar_div v a1) a2)]
+let rec vec_scalar_mul_zero_scalar (#o: orient) (#n: pos) (v: vec o n) (a: num)
+    : Lemma (requires is_zero a)
+      (ensures is_zero_vec (vec_scalar_mul v a))
+      [SMTPat (vec_scalar_mul v a)] =
+  match v with
+  | Vec1 _ -> ()
+  | VecN v' _ -> vec_scalar_mul_zero_scalar v' a
+
+(* vector-scalar div *)
+let rec vec_scalar_div (#o: orient) (#n: pos) (v: vec o n) (a: num{is_nnz a}) : vec o n =
+  match v with
+  | Vec1 x -> Vec1 (scalar_div x a)
+  | VecN v' x -> VecN (vec_scalar_div v' a) (scalar_div x a)
+
+let rec vec_scalar_div_assoc (#o: orient) (#n: pos) (v: vec o n)
+      (a1: num{is_nnz a1}) (a2: num{is_nnz a2})
+    : Lemma (vec_scalar_div (vec_scalar_div v a1) a2 == vec_scalar_div v (scalar_mul a1 a2))
+      [SMTPat (vec_scalar_div (vec_scalar_div v a1) a2)] =
+  match v with
+  | Vec1 _ -> ()
+  | VecN v' _ -> vec_scalar_div_assoc v' a1 a2
+
+let rec vec_scalar_div_mul (#o: orient) (#n: pos) (v: vec o n) (a: num{is_nnz a})
+    : Lemma (vec_scalar_mul (vec_scalar_div v a) a == v)
+      [SMTPat (vec_scalar_mul (vec_scalar_div v a) a)] =
+  match v with
+  | Vec1 _ -> ()
+  | VecN v' _ -> vec_scalar_div_mul v' a
 
 (* inner product *)
-assume val inner_prod : #n:pos -> rvec n -> cvec n -> num
+let rec inner_prod (#n: pos) (r: rvec n) (c: cvec n) : num =
+  match r with
+  | Vec1 x -> let Vec1 y = c in scalar_mul x y
+  | VecN r' rx -> let VecN c' cy = c in scalar_add (inner_prod r' c') (scalar_mul rx cy)
 
-assume val inner_prod_zero : #n:pos -> r:rvec n -> c:cvec n ->
-  Lemma (requires zero_vec r \/ zero_vec c) (ensures zero (inner_prod r c)) 
-  [SMTPat (inner_prod r c)]
+let rec inner_prod_zero (#n: pos) (r: rvec n) (c: cvec n)
+    : Lemma (requires is_zero_vec r \/ is_zero_vec c) (ensures is_zero (inner_prod r c))
+      [SMTPat (inner_prod r c)] =
+  match r with
+  | Vec1 _ -> let Vec1 _ = c in ()
+  | VecN r' _ -> let VecN c' _ = c in inner_prod_zero r' c'
 
 (* transpose vector *)
-assume val trans_vec : #n:pos -> v1:vec n -> v2:vec n{
-  (row v1 ==> col v2 ) /\ (col v1 ==> row v2) /\
-  (zero_vec v1 ==> zero_vec v2)
-}
+let rec vec_trans (#o: orient) (#n: pos) (v: vec o n) : vec (flip o) n =
+  match v with
+  | Vec1 x -> Vec1 x
+  | VecN v' x -> VecN (vec_trans v') x
 
-assume val trans_vec_scalar_div : #n:pos -> v:vec n -> a:num{nnz a} ->
-  Lemma (trans_vec (vec_scalar_div v a) == vec_scalar_div (trans_vec v) a)
-        [SMTPat (trans_vec (vec_scalar_div v a))]
+let rec vec_trans_zero (#o: orient) (#n: pos) (v: vec o n)
+    : Lemma (requires is_zero_vec v) (ensures is_zero_vec (vec_trans v)) [SMTPat (vec_trans v)] =
+  match v with
+  | Vec1 _ -> ()
+  | VecN v' _ -> vec_trans_zero v'
+
+let rec vec_trans_scalar_div (#o: orient) (#n: pos) (v: vec o n) (a: num{is_nnz a})
+    : Lemma (vec_trans (vec_scalar_div v a) == vec_scalar_div (vec_trans v) a)
+      [SMTPat (vec_trans (vec_scalar_div v a))] =
+  match v with
+  | Vec1 _ -> ()
+  | VecN v' _ -> vec_trans_scalar_div v' a
+  
+let rec vec_trans_involutive (#o: orient) (#n: pos) (v: vec o n)
+    : Lemma (vec_trans (vec_trans v) == v) [SMTPat (vec_trans (vec_trans v))] =
+  match v with
+  | Vec1 _ -> ()
+  | VecN v' _ -> vec_trans_involutive v'
