programs/LU.fst
@@ -5,13 +5,12 @@ open All
 let rec lu (#n:pos) (m:mat n{rowsdd m \/ spd m}) :
   l:mat n{unit_lower l} &
   u:mat n{upper u /\ nnz_diag u /\ mat_mul l u == m} =
-  match n with
-  | 1 -> (|_id_mat #1, m|)
-  | _ ->
-    let (|c, a, b, d|) = destruct m in
+  match m with
+  | Mat1 a -> (|id_mat, m|)
+  | MatN d c a b ->
     let s = schur1 d c a b in
     let (|l, u|) = lu s in
     let lc = vec_scalar_div c a in
-    let l' = augment l lc _one _zero_rvec in
-    let u' = augment u _zero_cvec a b in
+    let l' = MatN l lc one zero_rvec in
+    let u' = MatN u zero_cvec a b in
     (|l', u'|)
