programs/Solve.fst
@@ -3,7 +3,7 @@ module Solve
 open All
 open TriInv
 
-let solve (#n:pos) (l:mat n{unit_lower l}) (b:cvec n) : 
+let solve (#n:pos) (l:mat n{unit_lower l}) (b:cvec n) :
     x:cvec n{mat_vec_mul l x == b} =
     let l_inv = triangular_inv l in
     mat_vec_mul l_inv b
